merge

Examples/FAISpec.v
@@ -3,21 +3,65 @@ From LHL.Core Require Import
   Traces
   Program.
 
+From LHL.Util Require Import
+  Tactics
+  Util.
+
 Variant FAISig : ESig :=
 | FAI : FAISig nat.
 
-Definition FAIState : Type := nat * option ThreadName.
-Definition FAIIdle n : FAIState := (n, None).
-Definition FAIRan i n : FAIState := (n, Some i).
+Definition FAIState T : Type := nat * option (Name T).
+Notation FAIIdle n := (n, None).
+Notation FAIRan i n := (n, Some i).
 
-Variant FAIStep : FAIState -> ThreadEvent FAISig -> FAIState -> Prop :=
+Variant FAIStep {T} : FAIState T -> ThreadEvent T FAISig -> FAIState T -> Prop :=
 | FAICall i n : FAIStep (FAIIdle n) (i, CallEv FAI) (FAIRan i n)
 | FAIRet i n : FAIStep (FAIRan i n) (i, RetEv FAI n) (FAIIdle (S n)).
 
-Program Definition faiSpec : Spec FAISig := {|
-  State := FAIState;
+Require Import Coq.Program.Wf.
+Require Import Lia.
+
+Program Fixpoint faiSC {T} s
+  (p : list (ThreadEvent T FAISig)) (n : nat) {measure (length p)}
+: TransUtil.Steps FAIStep (FAIIdle n) p s ->
+  SeqConsistent (fun _ : Name T => None) p
+:= _.
+Next Obligation.
+Proof.
+  ddestruct H. constructor.
+  ddestruct H.
+  eapply SCCall with
+    (a':=fun j =>
+      if i =? j then
+        Some (existT _ _ FAI)
+      else
+        None).
+  { easy. }
+  { now rewrite eqb_id. }
+  { apply differ_pointwise_trivial. }
+  ddestruct H0. constructor.
+  ddestruct H.
+  eapply SCRet with
+    (a':=fun _ => None).
+  { now rewrite eqb_id. }
+  { easy. }
+  {
+    unfold differ_pointwise.
+    intros. now rewrite eqb_nid.
+  }
+  eapply faiSC.
+  { simpl. lia. }
+  { exact H0. }
+Qed.
+
+Program Definition faiSpec {T} : Spec T FAISig := {|
+  State := FAIState T;
   Step := FAIStep;
   Init := FAIIdle 0
 |}.
 
-Admit Obligations.
+Next Obligation.
+Proof.
+  eapply faiSC.
+  exact H.
+Qed.
