Examples/Counter/CounterSig.v
@@ -1,0 +1,6 @@
+From LHL.Core Require Import
+  Program.
+
+Variant CounterSig : ESig :=
+| Inc : CounterSig unit
+| Get : CounterSig nat.
